Capless/Renaming/Capture/Subtyping.lean
@@ -44,6 +44,14 @@ theorem SSubtyp.crename
     rename_i ih _ _ _ _
     apply ih; try assumption
     apply CVarMap.cext <;> trivial
+  case existp_erase =>
+    unfold crename_motive1 crename_motive2
+    repeat intro
+    simp [EType.crename]
+    apply ESubtyp.existp_erase
+    rename_i ih _ _ _ _
+    apply ih; try assumption
+    apply CVarMap.cext <;> trivial
   case type =>
     unfold crename_motive2 crename_motive1
     repeat intro
@@ -151,6 +159,11 @@ theorem ESubtyp.crename
   case exist hc =>
     simp [EType.crename]
     apply ESubtyp.exist
+    apply CSubtyp.crename; trivial
+    apply ρ.cext
+  case existp_erase =>
+    simp [EType.crename]
+    apply existp_erase
     apply CSubtyp.crename; trivial
     apply ρ.cext
   case type =>
