Capless/Renaming/Term/Subcapturing.lean
@@ -44,5 +44,15 @@ theorem Subcapt.rename
     simp [CBinding.rename] at hb1
     apply cinstr
     assumption
+  case reachl hb =>
+    simp [CaptureSet.rename_csingleton, CaptureSet.rename_rsingleton]
+    have hb1 := ρ.map _ _ hb
+    simp [EType.rename] at hb1
+    apply reachl; trivial
+  case reachr hb =>
+    simp [CaptureSet.rename_csingleton, CaptureSet.rename_rsingleton]
+    have hb1 := ρ.map _ _ hb
+    simp [EType.rename] at hb1
+    apply reachr; trivial
 
 end Capless
