Capless/Subcapturing.lean
@@ -27,5 +27,11 @@ inductive Subcapt : Context n m k -> CaptureSet n k -> CaptureSet n k -> Prop wh
 | cinstr :
   Context.CBound Γ c (CBinding.inst C) ->
   Subcapt Γ (CaptureSet.csingleton c) C
+| reachl :
+  Context.Bound Γ x (EType.exp c T) ->
+  Subcapt Γ (CaptureSet.csingleton c) (CaptureSet.rsingleton x)
+| reachr :
+  Context.Bound Γ x (EType.exp c T) ->
+  Subcapt Γ (CaptureSet.rsingleton x) (CaptureSet.csingleton c)
 
 end Capless
